Hnr_Array.thy
@@ -51,10 +51,10 @@ lemma hnr_copy_arr [hnr_rule_arr]:
   "hnr (array_assn x xi) (return xi) array_assn x"
   using hnr_pass by fastforce
 
-method refl = rule ent_refl
+method ent_refl = rule ent_refl
 
-method hnr_arr = hnr refl refl rule_set: hnr_rule_arr
+method hnr_arr = hnr ent_refl ent_refl rule_set: hnr_rule_arr
 
-method hnr_step_arr = hnr_step refl refl rule_set: hnr_rule_arr
+method hnr_step_arr = hnr_step ent_refl ent_refl rule_set: hnr_rule_arr
 
 end
